ocaml-cheerios/bit_vector.mli
@@ -6,6 +6,9 @@ val makeWriter : unit -> writer
 val pushBack : writer -> char -> unit
 val pop : reader -> char
 
+val writerToBytes : writer -> bytes
+val bytesToReader : bytes -> reader
+
 (* for testing *)
 val numBytes : writer -> int
 val writerToReader : writer -> reader
